Move lemmas to their appropriate places

pcuic/theories/PCUICConversion.v
@@ -2553,6 +2553,23 @@ Proof.
   all:typeclasses eauto.
 Qed.
 
+Lemma R_global_instance_length Σ Req Rle ref napp i i' :  
+  R_global_instance Σ Req Rle ref napp i i' -> #|i| = #|i'|.
+Proof.
+  unfold R_global_instance.
+  destruct global_variance.
+  { induction i in l, i' |- *; destruct l, i'; simpl; auto; try easy. }
+  { unfold R_universe_instance. 
+    intros H % Forall2_length. now rewrite !map_length in H. }
+Qed.
+
+Lemma R_universe_instance_variance_irrelevant Re Rle i i' :
+  #|i| = #|i'| ->
+  R_universe_instance_variance Re Rle [] i i'.
+Proof.
+  now induction i in i' |- *; destruct i'; simpl; auto.
+Qed.
+
 Lemma weakening_conv_gen :
   forall {cf : checker_flags} (Σ : global_env × universes_decl)
     (Γ Γ' Γ'' : PCUICAst.context) (M N : term) k,
@@ -2603,4 +2620,174 @@ Proof.
         simpl. intros * X. rewrite !app_context_assoc in X.
         destruct X; constructor; auto.
       * now rewrite app_context_assoc in HB.
+Qed.
+
+Require Import CMorphisms.
+Notation conv_terms Σ Γ := (All2 (conv Σ Γ)).
+
+Instance conv_terms_Proper {cf:checker_flags} Σ Γ : CMorphisms.Proper (eq ==> eq ==> arrow)%signature (conv_terms Σ Γ).
+Proof. intros x y -> x' y' -> f. exact f. Qed.
+
+Definition conv_ctx_rel {cf:checker_flags} Σ Γ Δ Δ' :=
+  All2_local_env (on_decl (fun Γ' _ x y => Σ ;;; Γ ,,, Γ' |- x = y)) Δ Δ'.
+
+Definition cumul_ctx_rel {cf:checker_flags} Σ Γ Δ Δ' :=
+  All2_local_env (on_decl (fun Γ' _ x y => Σ ;;; Γ ,,, Γ' |- x <= y)) Δ Δ'.
+
+Lemma cumul_subst_conv {cf:checker_flags} (Σ : global_env_ext) Γ Δ Δ' Γ' s s' b : wf Σ ->
+  All2 (conv Σ Γ) s s' ->
+  untyped_subslet Γ s Δ ->
+  untyped_subslet Γ s' Δ' ->
+  cumul Σ (Γ ,,, Γ') (subst s #|Γ'| b) (subst s' #|Γ'| b).
+Proof.
+  move=> wfΣ eqsub subs subs'.
+  eapply conv_cumul. eapply conv_subst_conv; eauto.
+Qed.
+
+Lemma subst_cumul {cf:checker_flags} {Σ} Γ Γ0 Γ1 Δ s s' T U : 
+  wf Σ.1 ->
+  subslet Σ Γ s Γ0 ->
+  subslet Σ Γ s' Γ1 ->
+  All2 (conv Σ Γ) s s' ->
+  wf_local Σ (Γ ,,, Γ0 ,,, Δ) ->
+  Σ;;; Γ ,,, Γ0 ,,, Δ |- T <= U ->
+  Σ;;; Γ ,,, subst_context s 0 Δ |- subst s #|Δ| T <= subst s' #|Δ| U.
+Proof.
+  move=> wfΣ subss subss' eqsub wfctx eqty.
+  eapply cumul_trans => //.
+  * eapply substitution_cumul => //.
+  ** eauto.
+  ** auto. 
+  ** eapply eqty.
+  * clear eqty.
+    rewrite -(subst_context_length s 0 Δ).
+    eapply cumul_subst_conv => //; eauto using subslet_untyped_subslet.
+Qed.
+
+Lemma untyped_subst_cumul {cf:checker_flags} {Σ} Γ Γ0 Γ1 Δ s s' T U : 
+  wf Σ.1 ->
+  untyped_subslet Γ s Γ0 ->
+  untyped_subslet Γ s' Γ1 ->
+  All2 (conv Σ Γ) s s' ->
+  wf_local Σ (Γ ,,, Γ0 ,,, Δ) ->
+  Σ;;; Γ ,,, Γ0 ,,, Δ |- T <= U ->
+  Σ;;; Γ ,,, subst_context s 0 Δ |- subst s #|Δ| T <= subst s' #|Δ| U.
+Proof.
+  move=> wfΣ subss subss' eqsub wfctx eqty.
+  eapply cumul_trans => //.
+  * eapply substitution_untyped_cumul => //.
+  ** eauto. 
+  ** eapply eqty.
+  * clear eqty.
+    rewrite -(subst_context_length s 0 Δ).
+    eapply cumul_subst_conv => //; eauto using subslet_untyped_subslet.
+Qed.
+
+Lemma conv_ctx_subst {cf:checker_flags} Σ Γ Γ' Δ Δ' s s' : 
+  wf Σ.1 ->
+  wf_local Σ (Γ ,,, Γ' ,,, Δ) ->
+  conv_ctx_rel Σ (Γ ,,, Γ') Δ Δ' ->
+  All2 (conv Σ []) s s' ->
+  subslet Σ [] s Γ ->
+  subslet Σ [] s' Γ ->
+  conv_ctx_rel Σ (subst_context s 0 Γ') (subst_context s #|Γ'| Δ) (subst_context s' #|Γ'| Δ').
+Proof.
+  intros wfΣ wf. induction 1.
+  - simpl. constructor.
+  - rewrite !subst_context_snoc /=.
+    intros Hs subs subs'.
+    depelim wf; simpl in H; noconf H.
+    specialize (IHX wf Hs subs subs').
+    constructor; auto.
+    red. red in p. simpl.
+    epose proof (subst_conv [] Γ Γ (Γ' ,,, Γ0) _ _ _ _ wfΣ subs subs' Hs).
+    rewrite app_context_nil_l app_context_assoc in X0.
+    specialize (X0 wf p).
+    rewrite subst_context_app in X0; autorewrite with len in X0.
+    rewrite app_context_nil_l in X0.
+    now rewrite -(All2_local_env_length X).
+  - rewrite !subst_context_snoc /=.
+    intros Hs subs subs'.
+    depelim wf; simpl in H; noconf H.
+    specialize (IHX wf Hs subs subs').
+    constructor; auto.
+    red. red in p. simpl.
+    destruct p as [pb pt].
+    epose proof (subst_conv [] Γ Γ (Γ' ,,, Γ0) _ _ _ _ wfΣ subs subs' Hs) as X0.
+    rewrite app_context_nil_l app_context_assoc in X0.
+    specialize (X0 wf pb).
+    epose proof (subst_conv [] Γ Γ (Γ' ,,, Γ0) _ _ _ _ wfΣ subs subs' Hs) as X1.
+    rewrite app_context_nil_l app_context_assoc in X1.
+    specialize (X1 wf pt).
+    rewrite !subst_context_app !app_context_nil_l in X0, X1; autorewrite with len in X0, X1.
+    now rewrite -(All2_local_env_length X).
+Qed.
+
+Lemma conv_terms_weaken {cf:checker_flags} Σ Γ Γ' args args' :
+  wf Σ.1 ->
+  wf_local Σ Γ ->
+  wf_local Σ Γ' ->
+  All (closedn #|Γ|) args -> All (closedn #|Γ|) args' ->
+  conv_terms Σ Γ args args' ->
+  conv_terms Σ (Γ' ,,, Γ) args args'.
+Proof.
+  intros wfΣ wf wf' cl cl' conv.
+  solve_all.
+  eapply weaken_conv; eauto.
+Qed.
+
+Lemma conv_terms_subst {cf:checker_flags} Σ Γ Γ' Γ'' Δ s s' args args' :
+  wf Σ.1 ->
+  wf_local Σ (Γ ,,, Γ' ,,, Δ) ->
+  subslet Σ Γ s Γ' ->
+  subslet Σ Γ s' Γ'' ->
+  conv_terms Σ Γ s s' ->
+  conv_terms Σ (Γ ,,, Γ' ,,, Δ) args args' ->
+  conv_terms Σ (Γ ,,, subst_context s 0 Δ) (map (subst s #|Δ|) args) (map (subst s' #|Δ|) args').
+Proof.
+  intros wfΣ wf cl cl' convs conv.
+  eapply All2_map.
+  eapply (All2_impl conv).
+  intros x y eqxy.
+  eapply subst_conv; eauto.
+Qed.
+
+Lemma cumul_ctx_subst {cf:checker_flags} Σ Γ Γ' Δ Δ' s s' : 
+  wf Σ.1 ->
+  wf_local Σ (Γ ,,, Γ' ,,, Δ) ->
+  cumul_ctx_rel Σ (Γ ,,, Γ') Δ Δ' ->
+  All2 (conv Σ []) s s' ->
+  subslet Σ [] s Γ ->
+  subslet Σ [] s' Γ ->
+  cumul_ctx_rel Σ (subst_context s 0 Γ') (subst_context s #|Γ'| Δ) (subst_context s' #|Γ'| Δ').
+Proof.
+  intros wfΣ wf. induction 1.
+  - simpl. constructor.
+  - rewrite !subst_context_snoc /=.
+    intros Hs subs subs'.
+    depelim wf; simpl in H; noconf H.
+    specialize (IHX wf Hs subs subs').
+    constructor; auto. 
+    red. red in p. simpl.
+    epose proof (subst_cumul [] Γ Γ (Γ' ,,, Γ0) _ _ _ _ wfΣ subs subs' Hs).
+    rewrite app_context_nil_l app_context_assoc in X0.
+    specialize (X0 wf p).
+    rewrite subst_context_app in X0; autorewrite with len in X0.
+    rewrite app_context_nil_l in X0.
+    now rewrite -(All2_local_env_length X).
+  - rewrite !subst_context_snoc /=.
+    intros Hs subs subs'.
+    depelim wf; simpl in H; noconf H.
+    specialize (IHX wf Hs subs subs').
+    constructor; auto.
+    red. red in p. simpl.
+    destruct p as [pb pt].
+    epose proof (subst_cumul [] Γ Γ (Γ' ,,, Γ0) _ _ _ _ wfΣ subs subs' Hs) as X0.
+    rewrite app_context_nil_l app_context_assoc in X0.
+    specialize (X0 wf pb).
+    epose proof (subst_cumul [] Γ Γ (Γ' ,,, Γ0) _ _ _ _ wfΣ subs subs' Hs) as X1.
+    rewrite app_context_nil_l app_context_assoc in X1.
+    specialize (X1 wf pt).
+    rewrite !subst_context_app !app_context_nil_l in X0, X1; autorewrite with len in X0, X1.
+    now rewrite -(All2_local_env_length X).
 Qed.
