pcuic/theories/PCUICSR.v
@@ -33,20 +33,12 @@ Arguments Universe.sort_of_product : simpl nomatch.
 Hint Rewrite subst_instance_context_assumptions : len.
 Hint Rewrite projs_length : len.
 
-Lemma nth_nth_error {A} {i} {l : list A} {d v} :
-  nth i l d = v ->
-  (nth_error l i = Some v) +
-  (nth_error l i = None /\ v = d).
-Proof.
-  move: i v. elim: l => [|hd tl IH] //.
-  - case => /= //; now right.
-  - case => /= // _ <-. now left.
-Qed.
-
 (** The subject reduction property of the system: *)
 
 Definition SR_red1 {cf:checker_flags} (Σ : global_env_ext) Γ t T :=
   forall u (Hu : red1 Σ Γ t u), Σ ;;; Γ |- u : T.
+
+(* Preservation of wf_*fixpoint *)  
 
 Lemma wf_fixpoint_red1_type {cf:checker_flags} (Σ : global_env_ext) Γ mfix mfix1 : 
   wf Σ.1 ->
@@ -170,358 +162,6 @@ Proof.
     simpl in *.
     noconf eqs. reflexivity.
   - simpl. now rewrite IHo.
-Qed.
-
-(** This shows that we can promote an argument spine for a given context to 
-    a spine for a context whose types are higher in the cumulativity relation.
-*)
-Lemma subslet_cumul {cf:checker_flags} Σ Δ args Γ Γ' : 
-  wf Σ.1 ->
-  assumption_context Γ -> assumption_context Γ' -> 
-  wf_local Σ (Δ ,,, Γ) ->
-  wf_local Σ (Δ ,,, Γ') ->
-  All2_local_env (fun Γ Γ' _ ty ty' => Σ ;;; Δ ,,, Γ |- ty <= ty') Γ Γ' ->
-  subslet Σ Δ args Γ -> subslet Σ Δ args Γ'.
-Proof.
-  intros wfΣ ass ass' wf wf' a2. induction a2 in wf, wf', args, ass, ass' |- *.
-  - inversion 1; constructor.
-  - intros subsl; depelim subsl; simpl in H; noconf H.
-    specialize (IHa2 s).
-    forward IHa2 by now depelim ass; simpl in H; noconf H.
-    forward IHa2 by now depelim ass'; simpl in H; noconf H.
-    depelim wf; simpl in H; noconf H.
-    depelim wf'; simpl in H; noconf H.
-    specialize (IHa2 wf wf' subsl).
-    constructor; auto.
-    eapply type_Cumul; eauto.
-    eapply isWAT_subst; eauto.
-    right; auto.
-    eapply (substitution_cumul _ _ _ []). eauto.
-    eapply wf. assumption. assumption.
-  - elimtype False; inv ass.
-Qed.
-
-Lemma spine_subst_cumul {cf:checker_flags} Σ Δ args Γ Γ' : 
-  wf Σ.1 ->
-  assumption_context Γ -> assumption_context Γ' -> 
-  wf_local Σ (Δ ,,, Γ) ->
-  wf_local Σ (Δ ,,, Γ') ->
-  All2_local_env (fun Γ Γ' _ ty ty' => Σ ;;; Δ ,,, Γ |- ty <= ty') Γ Γ' ->
-  spine_subst Σ Δ args (List.rev args) Γ -> 
-  spine_subst Σ Δ args (List.rev args) Γ'.
-Proof.
-  intros wfΣ ass ass' wf wf' a2.
-  intros []; split; auto.
-  - clear -a2 ass ass' inst_ctx_subst.
-    revert inst_ctx_subst; generalize (List.rev args).
-    intros l ctxs. 
-    induction ctxs in ass, Γ', ass', a2 |- *; depelim a2; try (simpl in H; noconf H); try constructor; auto.
-    * eapply IHctxs. now depelim ass.
-      now depelim ass'. auto.
-    * elimtype False; depelim ass. simpl in H; noconf H.
-  - eapply subslet_cumul. 6:eauto. all:eauto.
-Qed.
-
-Hint Resolve declared_inductive_minductive : core.
-
-Lemma context_assumptions_map f Γ : context_assumptions (map_context f Γ) = context_assumptions Γ.
-Proof.
-  induction Γ as [|[? [?|] ?] ?]; simpl; auto.
-Qed.
-
-Lemma subst_subst_lift (s s' : list term) n t : n = #|s| + #|s'| -> 
-  subst0 s (subst0 s' (lift0 n t)) = t.
-Proof.
-  intros ->. rewrite Nat.add_comm simpl_subst' //; try lia.
-  now rewrite -(Nat.add_0_r #|s|) simpl_subst' // lift0_id.
-Qed.
-
-Lemma All_refl {A} (P : A -> Type) l : (forall x, P x) -> All P l.
-Proof.
-  intros Hp; induction l; constructor; auto.
-Qed.
-
-Lemma map_subst_subst_lift_lift (s s' : list term) k k' l : k + k' = #|s| + #|s'| -> 
-  map (fun t => subst0 s (subst0 s' (lift k k' (lift0 k' t)))) l = l.
-Proof.
-  intros H. eapply All_map_id. eapply All_refl => x.
-  rewrite simpl_lift; try lia. rewrite subst_subst_lift //.
-Qed.
-
-Hint Rewrite context_assumptions_map : len.
-
-Lemma R_global_instance_length Σ Req Rle ref napp i i' :  
-  R_global_instance Σ Req Rle ref napp i i' -> #|i| = #|i'|.
-Proof.
-  unfold R_global_instance.
-  destruct global_variance.
-  { induction i in l, i' |- *; destruct l, i'; simpl; auto; try easy. }
-  { unfold R_universe_instance. 
-    intros H % Forall2_length. now rewrite !map_length in H. }
-Qed.
-
-Lemma R_universe_instance_variance_irrelevant Re Rle i i' :
-  #|i| = #|i'| ->
-  R_universe_instance_variance Re Rle [] i i'.
-Proof.
-  now induction i in i' |- *; destruct i'; simpl; auto.
-Qed.
-
-Lemma map_subst_extended_subst_lift_to_extended_list_k Γ :
- map (subst0 (extended_subst Γ 0)) (map (lift (context_assumptions Γ) #|Γ|)
-  (to_extended_list Γ)) = to_extended_list (smash_context [] Γ).
-Proof.
-  induction Γ as [|[na [b|] ty] ?]; simpl; auto.
-  rewrite (reln_lift 1).
-  rewrite -[reln [] 0 (smash_context [] Γ)]IHΓ.
-  rewrite !map_map_compose. apply map_ext => x.
-  rewrite -Nat.add_1_r -(permute_lift _ _ _ 1). lia.
-  rewrite (subst_app_decomp [_]).
-  rewrite simpl_subst_k /= //.
-  rewrite reln_acc (reln_lift 1) map_app /=.
-  rewrite smash_context_acc /= (reln_acc [tRel 0]) (reln_lift 1) map_app /=.
-  f_equal.
-  rewrite -[reln [] 0 (smash_context [] Γ)]IHΓ.
-  rewrite !map_map_compose. apply map_ext => x.
-  rewrite -(Nat.add_1_r #|Γ|) -(permute_lift _ _ _ 1). lia.
-  rewrite (subst_app_decomp [_]).
-  rewrite simpl_subst_k /= //.
-  rewrite lift_extended_subst.
-  rewrite distr_lift_subst. f_equal.
-  autorewrite with len. rewrite simpl_lift; lia_f_equal.
-Qed.
-
-Lemma All2_symmetry {A} (R : A -> A -> Type) : 
-  CRelationClasses.Symmetric R ->
-  CRelationClasses.Symmetric (All2 R).
-Proof.
-  intros HR x y l. 
-  induction l; constructor; auto.
-Qed.
-
-Lemma All2_transitivity {A} (R : A -> A -> Type) :
-  CRelationClasses.Transitive R ->
-  CRelationClasses.Transitive (All2 R).
-Proof.
-  intros HR x y z l; induction l in z |- *; auto.
-  intros H; depelim H. constructor; eauto.
-Qed.
-
-Definition conv_ctx_rel {cf:checker_flags} Σ Γ Δ Δ' :=
-  All2_local_env (on_decl (fun Γ' _ x y => Σ ;;; Γ ,,, Γ' |- x = y)) Δ Δ'.
-
-Definition cumul_ctx_rel {cf:checker_flags} Σ Γ Δ Δ' :=
-  All2_local_env (on_decl (fun Γ' _ x y => Σ ;;; Γ ,,, Γ' |- x <= y)) Δ Δ'.
-
-Lemma cumul_subst_conv {cf:checker_flags} (Σ : global_env_ext) Γ Δ Δ' Γ' s s' b : wf Σ ->
-  All2 (conv Σ Γ) s s' ->
-  untyped_subslet Γ s Δ ->
-  untyped_subslet Γ s' Δ' ->
-  cumul Σ (Γ ,,, Γ') (subst s #|Γ'| b) (subst s' #|Γ'| b).
-Proof.
-  move=> wfΣ eqsub subs subs'.
-  eapply conv_cumul. eapply conv_subst_conv; eauto.
-Qed.
-
-Lemma subst_cumul {cf:checker_flags} {Σ} Γ Γ0 Γ1 Δ s s' T U : 
-  wf Σ.1 ->
-  subslet Σ Γ s Γ0 ->
-  subslet Σ Γ s' Γ1 ->
-  All2 (conv Σ Γ) s s' ->
-  wf_local Σ (Γ ,,, Γ0 ,,, Δ) ->
-  Σ;;; Γ ,,, Γ0 ,,, Δ |- T <= U ->
-  Σ;;; Γ ,,, subst_context s 0 Δ |- subst s #|Δ| T <= subst s' #|Δ| U.
-Proof.
-  move=> wfΣ subss subss' eqsub wfctx eqty.
-  eapply cumul_trans => //.
-  * eapply substitution_cumul => //.
-  ** eauto.
-  ** auto. 
-  ** eapply eqty.
-  * clear eqty.
-    rewrite -(subst_context_length s 0 Δ).
-    eapply cumul_subst_conv => //; eauto using subslet_untyped_subslet.
-Qed.
-
-Lemma untyped_subst_cumul {cf:checker_flags} {Σ} Γ Γ0 Γ1 Δ s s' T U : 
-  wf Σ.1 ->
-  untyped_subslet Γ s Γ0 ->
-  untyped_subslet Γ s' Γ1 ->
-  All2 (conv Σ Γ) s s' ->
-  wf_local Σ (Γ ,,, Γ0 ,,, Δ) ->
-  Σ;;; Γ ,,, Γ0 ,,, Δ |- T <= U ->
-  Σ;;; Γ ,,, subst_context s 0 Δ |- subst s #|Δ| T <= subst s' #|Δ| U.
-Proof.
-  move=> wfΣ subss subss' eqsub wfctx eqty.
-  eapply cumul_trans => //.
-  * eapply substitution_untyped_cumul => //.
-  ** eauto. 
-  ** eapply eqty.
-  * clear eqty.
-    rewrite -(subst_context_length s 0 Δ).
-    eapply cumul_subst_conv => //; eauto using subslet_untyped_subslet.
-Qed.
-
-Lemma conv_ctx_subst {cf:checker_flags} Σ Γ Γ' Δ Δ' s s' : 
-  wf Σ.1 ->
-  wf_local Σ (Γ ,,, Γ' ,,, Δ) ->
-  conv_ctx_rel Σ (Γ ,,, Γ') Δ Δ' ->
-  All2 (conv Σ []) s s' ->
-  subslet Σ [] s Γ ->
-  subslet Σ [] s' Γ ->
-  conv_ctx_rel Σ (subst_context s 0 Γ') (subst_context s #|Γ'| Δ) (subst_context s' #|Γ'| Δ').
-Proof.
-  intros wfΣ wf. induction 1.
-  - simpl. constructor.
-  - rewrite !subst_context_snoc /=.
-    intros Hs subs subs'.
-    depelim wf; simpl in H; noconf H.
-    specialize (IHX wf Hs subs subs').
-    constructor. apply IHX.
-    red. red in p. simpl.
-    epose proof (subst_conv [] Γ Γ (Γ' ,,, Γ0) _ _ _ _ wfΣ subs subs' Hs).
-    rewrite app_context_nil_l app_context_assoc in X0.
-    specialize (X0 wf p).
-    rewrite subst_context_app in X0; autorewrite with len in X0.
-    rewrite app_context_nil_l in X0.
-    now rewrite -(All2_local_env_length X).
-  - rewrite !subst_context_snoc /=.
-    intros Hs subs subs'.
-    depelim wf; simpl in H; noconf H.
-    specialize (IHX wf Hs subs subs').
-    constructor. apply IHX.
-    red. red in p. simpl.
-    destruct p as [pb pt].
-    epose proof (subst_conv [] Γ Γ (Γ' ,,, Γ0) _ _ _ _ wfΣ subs subs' Hs) as X0.
-    rewrite app_context_nil_l app_context_assoc in X0.
-    specialize (X0 wf pb).
-    epose proof (subst_conv [] Γ Γ (Γ' ,,, Γ0) _ _ _ _ wfΣ subs subs' Hs) as X1.
-    rewrite app_context_nil_l app_context_assoc in X1.
-    specialize (X1 wf pt).
-    rewrite !subst_context_app !app_context_nil_l in X0, X1; autorewrite with len in X0, X1.
-    now rewrite -(All2_local_env_length X).
-Qed.
- 
-
-Notation conv_terms Σ Γ := (All2 (conv Σ Γ)).
-
-Lemma conv_terms_weaken {cf:checker_flags} Σ Γ Γ' args args' :
-  wf Σ.1 ->
-  wf_local Σ Γ ->
-  wf_local Σ Γ' ->
-  All (closedn #|Γ|) args -> All (closedn #|Γ|) args' ->
-  conv_terms Σ Γ args args' ->
-  conv_terms Σ (Γ' ,,, Γ) args args'.
-Proof.
-  intros wfΣ wf wf' cl cl' conv.
-  solve_all.
-  eapply weaken_conv; eauto.
-Qed.
-
-Lemma conv_terms_subst {cf:checker_flags} Σ Γ Γ' Γ'' Δ s s' args args' :
-  wf Σ.1 ->
-  wf_local Σ (Γ ,,, Γ' ,,, Δ) ->
-  subslet Σ Γ s Γ' ->
-  subslet Σ Γ s' Γ'' ->
-  conv_terms Σ Γ s s' ->
-  conv_terms Σ (Γ ,,, Γ' ,,, Δ) args args' ->
-  conv_terms Σ (Γ ,,, subst_context s 0 Δ) (map (subst s #|Δ|) args) (map (subst s' #|Δ|) args').
-Proof.
-  intros wfΣ wf cl cl' convs conv.
-  eapply All2_map.
-  eapply (All2_impl conv).
-  intros x y eqxy.
-  eapply subst_conv; eauto.
-Qed.
-
-Lemma to_extended_list_k_lift_context c k n k' : 
-  to_extended_list_k (lift_context n k c) k' = to_extended_list_k c k'. 
-Proof. now rewrite to_extended_list_k_fold_context. Qed.
-
-Lemma cumul_ctx_subst {cf:checker_flags} Σ Γ Γ' Δ Δ' s s' : 
-  wf Σ.1 ->
-  wf_local Σ (Γ ,,, Γ' ,,, Δ) ->
-  cumul_ctx_rel Σ (Γ ,,, Γ') Δ Δ' ->
-  All2 (conv Σ []) s s' ->
-  subslet Σ [] s Γ ->
-  subslet Σ [] s' Γ ->
-  cumul_ctx_rel Σ (subst_context s 0 Γ') (subst_context s #|Γ'| Δ) (subst_context s' #|Γ'| Δ').
-Proof.
-  intros wfΣ wf. induction 1.
-  - simpl. constructor.
-  - rewrite !subst_context_snoc /=.
-    intros Hs subs subs'.
-    depelim wf; simpl in H; noconf H.
-    specialize (IHX wf Hs subs subs').
-    constructor. apply IHX.
-    red. red in p. simpl.
-    epose proof (subst_cumul [] Γ Γ (Γ' ,,, Γ0) _ _ _ _ wfΣ subs subs' Hs).
-    rewrite app_context_nil_l app_context_assoc in X0.
-    specialize (X0 wf p).
-    rewrite subst_context_app in X0; autorewrite with len in X0.
-    rewrite app_context_nil_l in X0.
-    now rewrite -(All2_local_env_length X).
-  - rewrite !subst_context_snoc /=.
-    intros Hs subs subs'.
-    depelim wf; simpl in H; noconf H.
-    specialize (IHX wf Hs subs subs').
-    constructor. apply IHX.
-    red. red in p. simpl.
-    destruct p as [pb pt].
-    epose proof (subst_cumul [] Γ Γ (Γ' ,,, Γ0) _ _ _ _ wfΣ subs subs' Hs) as X0.
-    rewrite app_context_nil_l app_context_assoc in X0.
-    specialize (X0 wf pb).
-    epose proof (subst_cumul [] Γ Γ (Γ' ,,, Γ0) _ _ _ _ wfΣ subs subs' Hs) as X1.
-    rewrite app_context_nil_l app_context_assoc in X1.
-    specialize (X1 wf pt).
-    rewrite !subst_context_app !app_context_nil_l in X0, X1; autorewrite with len in X0, X1.
-    now rewrite -(All2_local_env_length X).
-Qed.
-
-Require Import CMorphisms.
-
-Instance conv_terms_Proper {cf:checker_flags} Σ Γ : CMorphisms.Proper (eq ==> eq ==> arrow)%signature (conv_terms Σ Γ).
-Proof. intros x y -> x' y' -> f. exact f. Qed.
-
-Lemma typing_spine_eq {cf:checker_flags} Σ Γ ty s s' ty' :
-  s = s' ->
-  typing_spine Σ Γ ty s ty' ->
-  typing_spine Σ Γ ty s' ty'.
-Proof. now intros ->. Qed.
-
-Lemma spine_subst_eq_target {cf:checker_flags} {Σ Γ s inst Δ Δ'} :
-  spine_subst Σ Γ s inst Δ ->
-  Δ = Δ' ->
-  spine_subst Σ Γ s inst Δ'.
-Proof. now intros H ->. Qed.
-
-Lemma arity_spine_it_mkProd_or_LetIn_Sort {cf:checker_flags} Σ Γ ctx s args inst : 
-  wf Σ.1 ->
-  spine_subst Σ Γ args inst ctx ->
-  arity_spine Σ Γ (it_mkProd_or_LetIn ctx (tSort s)) args (tSort s).
-Proof.
-  intros wfΣ sp. rewrite -(app_nil_r args).
-  eapply arity_spine_it_mkProd_or_LetIn => //.
-  eauto. constructor. left. eexists _, _; intuition eauto.
-  eapply sp. simpl. reflexivity.
-Qed.
-
-Lemma context_assumptions_mapi f Γ : context_assumptions (mapi (fun i => map_decl (f i)) Γ) = 
-  context_assumptions Γ.
-Proof.
-  rewrite /mapi; generalize 0.
-  induction Γ; simpl; intros; eauto.
-  destruct a as [? [b|] ?]; simpl; auto.
-Qed.
-
-Lemma ctx_inst_length {cf:checker_flags} Σ Γ args Δ :
-  ctx_inst Σ Γ args Δ -> 
-  #|args| = context_assumptions Δ.
-Proof.
-  induction 1; simpl; auto.
-  rewrite /subst_telescope in IHX.
-  rewrite context_assumptions_mapi in IHX. congruence.
-  rewrite context_assumptions_mapi in IHX. congruence.
 Qed.
 
 Lemma sr_red1 {cf:checker_flags} :
@@ -681,7 +321,7 @@ Proof.
       [parsubst [csubst ptyeq]]. 2:exact oib. subst pty.
     destruct heq_map_option_out as [nargs [br [brty [[[Hbr Hbrty] brbrty] brtys]]]].
     unshelve eapply (branch_type_spec Σ.1) in brtys; eauto. 2:eapply on_declared_inductive; eauto.
-    destruct (nth_nth_error (@eq_refl _ (nth c0 brs (0, tDummy)))) => //.
+    destruct (nth_nth_error' (@eq_refl _ (nth c0 brs (0, tDummy)))) => //.
     2:{ simpl in Hbr. rewrite Hbr in a. intuition discriminate. }
     assert (H : ∑ t', nth_error btys c0 = Some t').
     pose proof (All2_length _ _ X5). eapply nth_error_Some_length in e. rewrite H in e.
@@ -810,7 +450,7 @@ Proof.
            rewrite subst_it_mkProd_or_LetIn.
            eapply arity_spine_it_mkProd_or_LetIn_Sort => //.
            simpl in sp. instantiate (1:=inst).
-           eapply spine_subst_eq_target; [eapply sp|].
+           eapply spine_subst_eq; [eapply sp|].
            rewrite distr_lift_subst_context -H. f_equal.
            rewrite -(context_subst_length _ _ _ iparsubst0).
            autorewrite with len. rewrite closed_ctx_lift //.
@@ -1844,7 +1484,6 @@ Section SRContext.
         rewrite !(simpl_lift0 _ (S n)).
         eapply (weakening_red_0 wfΣ _ [_]); tas; cbnr.
   Qed.
-
 
   Lemma wf_local_isType_nth Σ Γ n decl :
     wf Σ.1 ->
